@prefix : <https://w3id.org/pmd/hto/hto-simple.ttl#> .
@prefix obo: <http://purl.obolibrary.org/obo/> .
@prefix owl: <http://www.w3.org/2002/07/owl#> .
@prefix rdf: <http://www.w3.org/1999/02/22-rdf-syntax-ns#> .
@prefix xml: <http://www.w3.org/XML/1998/namespace> .
@prefix xsd: <http://www.w3.org/2001/XMLSchema#> .
@prefix rdfs: <http://www.w3.org/2000/01/rdf-schema#> .
@prefix skos: <http://www.w3.org/2004/02/skos/core#> .
@prefix terms: <http://purl.org/dc/terms/> .
@base <https://w3id.org/pmd/hto/hto-simple.ttl> .

<https://w3id.org/pmd/hto/hto-simple.ttl> rdf:type owl:Ontology ;
                                           owl:versionIRI <https://w3id.org/pmd/hto/releases/2025-11-28/hto-simple.ttl> ;
                                           terms:contributor "Jannis Grundmann" ;
                                           terms:creator <https://orcid.org/0000-0002-9014-2920> ,
                                                         <https://orcid.org/0000-0003-1649-6832> ,
                                                         <https://orcid.org/0009-0004-4787-4685> ;
                                           terms:description "This ontology module is part of the Platform Material Digital Application Ontology (PMDao) and covers concepts related to heat treatment processes, parameters, and materials. It is designed to facilitate data integration, sharing, and analysis in the field of materials science and engineering, particularly focusing on heat treatment applications."@en ;
                                           terms:license <https://creativecommons.org/licenses/unspecified> ;
                                           terms:title "Platform Material Digital Application Ontology (PMDao) - Heat Treatment Module"@en ;
                                           owl:versionInfo "2025-11-28" .

#################################################################
#    Annotation properties
#################################################################

###  http://purl.obolibrary.org/obo/IAO_0000112
obo:IAO_0000112 rdf:type owl:AnnotationProperty .


###  http://purl.obolibrary.org/obo/IAO_0000114
obo:IAO_0000114 rdf:type owl:AnnotationProperty .


###  http://purl.obolibrary.org/obo/IAO_0000115
obo:IAO_0000115 rdf:type owl:AnnotationProperty ;
                obo:IAO_0000115 "The official definition, explaining the meaning of a class or property. Shall be Aristotelian, formalized and normalized. Can be augmented with colloquial definitions."@en ;
                obo:IAO_0000116 """2012-04-05: 
Barry Smith

The official OBI definition, explaining the meaning of a class or property: 'Shall be Aristotelian, formalized and normalized. Can be augmented with colloquial definitions'  is terrible.

Can you fix to something like:

A statement of necessary and sufficient conditions explaining the meaning of an expression referring to a class or property.

Alan Ruttenberg

Your proposed definition is a reasonable candidate, except that it is very common that necessary and sufficient conditions are not given. Mostly they are necessary, occasionally they are necessary and sufficient or just sufficient. Often they use terms that are not themselves defined and so they effectively can't be evaluated by those criteria. 

On the specifics of the proposed definition:

We don't have definitions of 'meaning' or 'expression' or 'property'. For 'reference' in the intended sense I think we use the term 'denotation'. For 'expression', I think we you mean symbol, or identifier. For 'meaning' it differs for class and property. For class we want documentation that let's the intended reader determine whether an entity is instance of the class, or not. For property we want documentation that let's the intended reader determine, given a pair of potential relata, whether the assertion that the relation holds is true. The 'intended reader' part suggests that we also specify who, we expect, would be able to understand the definition, and also generalizes over human and computer reader to include textual and logical definition. 

Personally, I am more comfortable weakening definition to documentation, with instructions as to what is desirable. 

We also have the outstanding issue of how to aim different definitions to different audiences. A clinical audience reading chebi wants a different sort of definition documentation/definition from a chemistry trained audience, and similarly there is a need for a definition that is adequate for an ontologist to work with."""@en ,
                                """2012-04-05: 
Barry Smith

The official OBI definition, explaining the meaning of a class or property: 'Shall be Aristotelian, formalized and normalized. Can be augmented with colloquial definitions'  is terrible.

Can you fix to something like:

A statement of necessary and sufficient conditions explaining the meaning of an expression referring to a class or property.

Alan Ruttenberg

Your proposed definition is a reasonable candidate, except that it is very common that necessary and sufficient conditions are not given. Mostly they are necessary, occasionally they are necessary and sufficient or just sufficient. Often they use terms that are not themselves defined and so they effectively can't be evaluated by those criteria. 

On the specifics of the proposed definition:

We don't have definitions of 'meaning' or 'expression' or 'property'. For 'reference' in the intended sense I think we use the term 'denotation'. For 'expression', I think we you mean symbol, or identifier. For 'meaning' it differs for class and property. For class we want documentation that let's the intended reader determine whether an entity is instance of the class, or not. For property we want documentation that let's the intended reader determine, given a pair of potential relata, whether the assertion that the relation holds is true. The 'intended reader' part suggests that we also specify who, we expect, would be able to understand the definition, and also generalizes over human and computer reader to include textual and logical definition. 

Personally, I am more comfortable weakening definition to documentation, with instructions as to what is desirable. 

We also have the outstanding issue of how to aim different definitions to different audiences. A clinical audience reading chebi wants a different sort of definition documentation/definition from a chemistry trained audience, and similarly there is a need for a definition that is adequate for an ontologist to work with.  """@en ;
                obo:IAO_0000119 "GROUP:OBI:<http://purl.obolibrary.org/obo/obi>"@en ;
                rdfs:label "definition" ,
                           "definition"@en .


###  http://purl.obolibrary.org/obo/IAO_0000116
obo:IAO_0000116 rdf:type owl:AnnotationProperty .


###  http://purl.obolibrary.org/obo/IAO_0000119
obo:IAO_0000119 rdf:type owl:AnnotationProperty .


###  http://purl.org/dc/terms/contributor
terms:contributor rdf:type owl:AnnotationProperty .


###  http://purl.org/dc/terms/creator
terms:creator rdf:type owl:AnnotationProperty .


###  http://purl.org/dc/terms/description
terms:description rdf:type owl:AnnotationProperty ;
                  rdfs:label "description" .


###  http://purl.org/dc/terms/license
terms:license rdf:type owl:AnnotationProperty ;
              rdfs:label "dcterms:license" ,
                         "license" .


###  http://purl.org/dc/terms/title
terms:title rdf:type owl:AnnotationProperty ;
            rdfs:label "title" .


###  http://www.w3.org/2004/02/skos/core#definition
skos:definition rdf:type owl:AnnotationProperty .


###  http://www.w3.org/2004/02/skos/core#example
skos:example rdf:type owl:AnnotationProperty .


###  http://www.w3.org/2004/02/skos/core#prefLabel
skos:prefLabel rdf:type owl:AnnotationProperty .


#################################################################
#    Object Properties
#################################################################

###  http://purl.obolibrary.org/obo/BFO_0000051
obo:BFO_0000051 rdf:type owl:ObjectProperty ;
                rdfs:subPropertyOf obo:BFO_0000051 ;
                rdf:type owl:TransitiveProperty ;
                obo:IAO_0000112 "my body has part my brain (continuant parthood, two material entities)"@en ,
                                "my stomach has part my stomach cavity (continuant parthood, material entity has part immaterial entity)"@en ,
                                "this year has part this day (occurrent parthood)"@en ;
                obo:IAO_0000115 "a core relation that holds between a whole and its part"@en ;
                obo:IAO_0000116 "Everything has itself as a part. Any part of any part of a thing is itself part of that thing. Two distinct things cannot have each other as a part."@en ,
                                "Occurrents are not subject to change and so parthood between occurrents holds for all the times that the part exists. Many continuants are subject to change, so parthood between continuants will only hold at certain times, but this is difficult to specify in OWL. See http://purl.obolibrary.org/obo/ro/docs/temporal-semantics/"@en ,
                                """Parthood requires the part and the whole to have compatible classes: only an occurrent have an occurrent as part; only a process can have a process as part; only a continuant can have a continuant as part; only an independent continuant can have an independent continuant as part; only a specifically dependent continuant can have a specifically dependent continuant as part; only a generically dependent continuant can have a generically dependent continuant as part. (This list is not exhaustive.)

A continuant cannot have an occurrent as part: use 'participates in'. An occurrent cannot have a continuant as part: use 'has participant'. An immaterial entity cannot have a material entity as part: use 'location of'. An independent continuant cannot have a specifically dependent continuant as part: use 'bearer of'. A specifically dependent continuant cannot have an independent continuant as part: use 'inheres in'."""@en ;
                rdfs:label "has part"@en .


###  http://purl.obolibrary.org/obo/BFO_0000197
obo:BFO_0000197 rdf:type owl:ObjectProperty .


###  http://purl.obolibrary.org/obo/IAO_0000039
obo:IAO_0000039 rdf:type owl:ObjectProperty ;
                rdfs:subPropertyOf obo:BFO_0000051 ;
                rdf:type owl:FunctionalProperty ;
                rdfs:label "has measurement unit label"@en .


###  http://purl.obolibrary.org/obo/IAO_0000136
obo:IAO_0000136 rdf:type owl:ObjectProperty ;
                obo:IAO_0000112 "This document is about information artifacts and their representations"@en ;
                obo:IAO_0000115 "A (currently) primitive relation that relates an information artifact to an entity."@en ;
                obo:IAO_0000116 """7/6/2009 Alan Ruttenberg. Following discussion with Jonathan Rees, and introduction of \"mentions\" relation. Weaken the is_about relationship to be primitive. 

We will try to build it back up by elaborating the various subproperties that are more precisely defined.

Some currently missing phenomena that should be considered \"about\" are predications - \"The only person who knows the answer is sitting beside me\" , Allegory, Satire, and other literary forms that can be topical without explicitly mentioning the topic."""@en ;
                obo:IAO_0000119 "Smith, Ceusters, Ruttenberg, 2000 years of philosophy"@en ;
                rdfs:label "is about"@en .


###  http://purl.obolibrary.org/obo/RO_0000057
obo:RO_0000057 rdf:type owl:ObjectProperty ;
               owl:propertyChainAxiom ( obo:BFO_0000051
                                        obo:RO_0000057
                                      ) ;
               obo:IAO_0000112 "this blood coagulation has participant this blood clot"@en ,
                               "this investigation has participant this investigator"@en ,
                               "this process has participant this input material (or this output material)"@en ;
               obo:IAO_0000115 "a relation between a process and a continuant, in which the continuant is somehow involved in the process"@en ;
               obo:IAO_0000116 "Has_participant is a primitive instance-level relation between a process, a continuant, and a time at which the continuant participates in some way in the process. The relation obtains, for example, when this particular process of oxygen exchange across this particular alveolar membrane has_participant this particular sample of hemoglobin at this particular time."@en ;
               rdfs:label "has participant"@en .


###  http://purl.obolibrary.org/obo/RO_0000085
obo:RO_0000085 rdf:type owl:ObjectProperty ;
               obo:IAO_0000112 "this enzyme has function this catalysis function (more colloquially: this enzyme has this catalysis function)"@en ;
               obo:IAO_0000115 "a relation between an independent continuant (the bearer) and a function, in which the function specifically depends on the bearer for its existence"@en ;
               obo:IAO_0000116 "A bearer can have many functions, and its functions can exist for different periods of time, but none of its functions can exist when the bearer does not exist. A function need not be realized at all the times that the function exists."@en ;
               rdfs:label "has function"@en .


###  https://w3id.org/pmd/co/PMD_0000009
<https://w3id.org/pmd/co/PMD_0000009> rdf:type owl:ObjectProperty ;
                                      rdfs:label "has process attribute"@de ;
                                      rdfs:seeAlso "has process attribute from OEO https://openenergyplatform.org/ontology/oeo/OEO_00000500"@en ;
                                      skos:definition "A relation between a process and a process attribute that depends on it."@en ;
                                      skos:example "Tensile testing process has process attribute tensile rate"@en .


###  https://w3id.org/pmd/co/PMD_0020127
<https://w3id.org/pmd/co/PMD_0020127> rdf:type owl:ObjectProperty ;
                                      rdfs:comment """Despite has characteristic from RO does not have any domain constraints, it is still not possible to directly connect an instance of a process with an instance of a SDC. 

First, SDC is dependent on a IC. As RO does not have \"bearer of\" object property, the \"has characteristic\" implies that the domain should be an IC. 

Second, characteristic of is a functional property. Thus, two triples SDC_1 characteristc of IC_1 and SDC_2  characteristc of Process_1 (where IC_1 participates in Process_1), cannot exist simultaneously. 
An example of such case can be \"Temperature of during the annealing process was 1000°C\". Temperature is an SDC of some participant of the annealing, however it is not clear whether it is an SDC of an oven or of a sample in the oven. If we assert triple Annealing--> has characteristic --> Temperature 1000°C, then the correct triple connecting temperature SDC with either oven or specimen cannot exist."""@en ;
                                      rdfs:label "refers to"@en ;
                                      skos:definition "a relation between a process attribute and an SDC of some participant in a process"@en ;
                                      skos:example "a relation to between a process attribute an a SDC of some participant in a process."@en .


#################################################################
#    Classes
#################################################################

###  https://w3id.org/pmd/hto/AccelleratedCooling
<https://w3id.org/pmd/hto/AccelleratedCooling> rdf:type owl:Class ;
                                               obo:IAO_0000114 "needs work" ;
                                               rdfs:comment "Achieved via convection only."@en ,
                                                            "so convection cooling is a function of a device, it could be realized in a cooling process. definatl needs a better name like acllerated convection cooling function, to be specific" ;
                                               rdfs:isDefinedBy <https://w3id.org/pmd/hto/> ;
                                               rdfs:label "accellerated cooling"@en ;
                                               skos:definition "Status of the cooling method active e.g., at the end of the nitriding process"@en .


###  https://w3id.org/pmd/hto/AcquisitionDate
<https://w3id.org/pmd/hto/AcquisitionDate> rdf:type owl:Class ;
                                           obo:IAO_0000114 "needs work" ;
                                           rdfs:comment "is a temperal instant!" ;
                                           rdfs:isDefinedBy <https://w3id.org/pmd/hto/> ;
                                           rdfs:label "acquisition date"@en ;
                                           skos:definition "The point in time a Process Node was commissioned (e.g., the purchase date, first day of use), represented in IEEE 1003 'Seconds since Epoch'. "@en .


###  https://w3id.org/pmd/hto/Annealing
<https://w3id.org/pmd/hto/Annealing> rdf:type owl:Class ;
                                     rdfs:isDefinedBy <https://w3id.org/pmd/hto/> ;
                                     rdfs:label "annealing"@en ;
                                     skos:definition "Heat treatment process with the scope to change the properties or microstructure of a sample or part. Typically no hardening is performed with this process."@en .


###  https://w3id.org/pmd/hto/Atmosphere
<https://w3id.org/pmd/hto/Atmosphere> rdf:type owl:Class ;
                                      rdfs:subClassOf <https://w3id.org/pmd/hto/Medium> ;
                                      rdfs:label "atmosphere"@en ;
                                      skos:definition "A surrounding influence or environment" .


###  https://w3id.org/pmd/hto/AtmospherePressure
<https://w3id.org/pmd/hto/AtmospherePressure> rdf:type owl:Class ;
                                              rdfs:comment "Effective atmosphere preasure in chamber to keep process save (must be 2-3 mbar above ambient prssure)"@en ,
                                                           "Parameter usually slightly higher than ambient pressure for open process to environment to prevent/reduce diffusion of oxygen into the furnace, e.g. by leckage, to avoid explosive or dangerous atmopheres, could be bar, mbar or Pa"@en ;
                                              rdfs:isDefinedBy <https://w3id.org/pmd/hto/> ;
                                              rdfs:label "atmosphere pressure"@en ;
                                              skos:definition "Parameter describing the intended atmosphere pressure inside a chamber. "@en .


###  https://w3id.org/pmd/hto/BelowAmbientPressure
<https://w3id.org/pmd/hto/BelowAmbientPressure> rdf:type owl:Class ;
                                                rdfs:isDefinedBy <https://w3id.org/pmd/hto/> ;
                                                rdfs:label "below ambient pressure"@en ;
                                                skos:definition "status of atmosphere: reduced pressure below ambient pressure "@en .


###  https://w3id.org/pmd/hto/CarbonPotential
<https://w3id.org/pmd/hto/CarbonPotential> rdf:type owl:Class ;
                                           rdfs:comment "Nitrocarburieren mit Kohlenstoffträger, aus Messwerten abgeleitet KC"@de ,
                                                        "See standard DIN 1310"@en ;
                                           rdfs:isDefinedBy <https://w3id.org/pmd/hto/> ;
                                           rdfs:label "carbon potential"@en ;
                                           skos:definition "Carbon content of a specimen of pure iron in equilibrium with a carbourizing medium under specific conditions."@en .


###  https://w3id.org/pmd/hto/Carburizing
<https://w3id.org/pmd/hto/Carburizing> rdf:type owl:Class ;
                                       rdfs:comment "Potentiell ableitbar mit bestimmten Fluss-Schwellenwerten"@de ;
                                       rdfs:isDefinedBy <https://w3id.org/pmd/hto/> ;
                                       rdfs:label "Aufkohlen"@de ,
                                                  "carburizing recipe"@en ;
                                       skos:definition "Heattreatment process with the scope to transfer carbon from the atmosphere to the component surface."@en ,
                                                       "Prozessschritt, während dessen Kohlenstoff aus der Atmosphäre an der Bauteiloberfläche übertragen wird"@de .


###  https://w3id.org/pmd/hto/Chamber
<https://w3id.org/pmd/hto/Chamber> rdf:type owl:Class ;
                                   obo:IAO_0000114 "needs work" ;
                                   rdfs:comment "moved to fiat object part. correct if every furnace has a chamber" ,
                                                "unklare Zuordnung innerhalb der \"spec. dep. continuants\". Eine Kammer existiert nur als Teil eines Gerätes (Device), könnte aber selbst noch einmal als independent continuant definiert werden, da sich in der Kammer Chargen, Gestelle, Thermoelemente etc. befinden."@de ;
                                   rdfs:isDefinedBy <https://w3id.org/pmd/hto/> ;
                                   rdfs:label "chamber"@en ;
                                   skos:definition "Systemboundary of a distinct Heattreatment Process. Typically includes medium (e.g., Helium or Vacuum)."@en .


###  https://w3id.org/pmd/hto/ChamberPressure
<https://w3id.org/pmd/hto/ChamberPressure> rdf:type owl:Class ;
                                           rdfs:subClassOf [ rdf:type owl:Restriction ;
                                                             owl:onProperty obo:BFO_0000197 ;
                                                             owl:someValuesFrom <https://w3id.org/pmd/hto/Chamber>
                                                           ] ;
                                           rdfs:comment "measured atmophere pressure in retort, measured using the vacuum sensor "@en ;
                                           rdfs:isDefinedBy <https://w3id.org/pmd/hto/> ;
                                           rdfs:label "chamber pressure"@en ;
                                           skos:definition "designated pressure in retort during evacuation phase pre to nitriding process or during low pressure nitriding process "@en .


###  https://w3id.org/pmd/hto/ChamberScope
<https://w3id.org/pmd/hto/ChamberScope> rdf:type owl:Class ;
                                        obo:IAO_0000114 "needs work" ;
                                        rdfs:comment "Sollte mit Unit-Volume (m^3) verbunden sein"@de ,
                                                     "The reason for obsoletion is that the term is not clearly defined and usage has been inconsistent." ,
                                                     "competly dont get that one" ;
                                        rdfs:isDefinedBy <https://w3id.org/pmd/hto/> ;
                                        rdfs:label "obsolete Wärmebehandlungsofenkammer"@de ,
                                                   "obsolete chamberscope"@en ;
                                        owl:deprecated "true"^^xsd:boolean ;
                                        skos:definition "Funktionale Ofenkammer."@de ,
                                                        "OBSOLETE. Functional furnace chamber."@en ,
                                                        """OBSOLETE. Position of the batch in a multi-chamber furnace
A specialization of hasProcessNodeComponent representing distinguishable heat treatment chambers of a furnaces.
can be: heating chamber / cooling chamber"""@en .


###  https://w3id.org/pmd/hto/CollectionInterfaceHint
<https://w3id.org/pmd/hto/CollectionInterfaceHint> rdf:type owl:Class ;
                                                   rdfs:isDefinedBy <https://w3id.org/pmd/hto/> ;
                                                   rdfs:label "collection interface hint"@en ;
                                                   skos:definition "A label in support of identifying a network interface and/or address used by a process node to provide primary data stored in ontologies "@en .


###  https://w3id.org/pmd/hto/ConcentrationH2
<https://w3id.org/pmd/hto/ConcentrationH2> rdf:type owl:Class ;
                                           rdfs:subClassOf <https://w3id.org/pmd/hto/FurnaceAtmosphere> ;
                                           rdfs:comment "Ammonia is usually intenionally induced;"@en ,
                                                        "Einzelne Werte durch auf das Molekül spezifizierte Messsonden."@de ,
                                                        "Hydrogen can be formed during decomposition of e.g. ammonia, acetylene or can be intenionally induced e.g. in forming gas." ,
                                                        "Might be calculated from model or measurement."@en ,
                                                        "Oxygen concentration in process gas composition, oxygen can be formed during decomposition of e.g. carbon monoxide or dioxide or can be intenionally induced e.g. as air, synthetic air or water or enters the furnace via leckage."@en ,
                                                        "Water concentration in process gas composition, if nominal water is intenionally induced; units could be e.g. mol/m³ or °C; signal could be in mA or mV or in vol.-% or °C (dew point)"@en ;
                                           rdfs:isDefinedBy <https://w3id.org/pmd/hto/> ;
                                           rdfs:label "concentration"@en ;
                                           skos:definition "Concentration in process gas composition; units could be e.g. mol/m³; signal could be in mA or mV or in vol.-%"@en .


###  https://w3id.org/pmd/hto/Controlled
<https://w3id.org/pmd/hto/Controlled> rdf:type owl:Class ;
                                      rdfs:comment "definition is not enough, what is controlled?" ;
                                      rdfs:isDefinedBy <https://w3id.org/pmd/hto/> ;
                                      rdfs:label "controlled"@en ;
                                      skos:definition "This Scope expresses that a :ValueObject is actively controlled during the process, e.g. a heating process where the temperature change is done in controlled intervals until the desired temperature is reached while an uncontrolled heating process would reach the desired temperature as fast as the furnace allows it to."@en .


###  https://w3id.org/pmd/hto/Convection
<https://w3id.org/pmd/hto/Convection> rdf:type owl:Class ;
                                      rdfs:comment "if its a device specification to run a heat up process by some spefiic mode of action, then pls change the definition" ;
                                      rdfs:isDefinedBy <https://w3id.org/pmd/hto/> ;
                                      rdfs:label "convection"@en ;
                                      skos:definition "konvection during heating, heating in atmosphere, not in vacuum "@en .


###  https://w3id.org/pmd/hto/DewPoint
<https://w3id.org/pmd/hto/DewPoint> rdf:type owl:Class ;
                                    rdfs:isDefinedBy <https://w3id.org/pmd/hto/> ;
                                    rdfs:label "dew point"@en ;
                                    skos:definition "dew point of the atmosphere, measured during process or calculated from lambda / oxygen probe signal "@en .


###  https://w3id.org/pmd/hto/DurationTillTargetTemperature
<https://w3id.org/pmd/hto/DurationTillTargetTemperature> rdf:type owl:Class ;
                                                         rdfs:comment "Erwärmdauer = Heizzeit + Durchwärmdauer"@de ,
                                                                      "Maß für die tatsächliche Dauer eines Erwärmvorgangs."@de ;
                                                         rdfs:isDefinedBy <https://w3id.org/pmd/hto/> ;
                                                         rdfs:label "Erwärmdauer"@de ,
                                                                    "duration till target temperature"@en ;
                                                         skos:definition "Measurement representing the actual duration of a heating procedure."@en .


###  https://w3id.org/pmd/hto/DurationToReachTargetTemperature
<https://w3id.org/pmd/hto/DurationToReachTargetTemperature> rdf:type owl:Class ;
                                                            rdfs:isDefinedBy <https://w3id.org/pmd/hto/> ;
                                                            rdfs:label "duration to reach target temperature"@en ;
                                                            skos:definition "Parameter representing a derived duration of a heat up segment (in hours, minutes or seconds) "@en .


###  https://w3id.org/pmd/hto/Fan
<https://w3id.org/pmd/hto/Fan> rdf:type owl:Class ;
                               rdfs:comment "not properly defined" .


###  https://w3id.org/pmd/hto/FanStateFast
<https://w3id.org/pmd/hto/FanStateFast> rdf:type owl:Class ;
                                        obo:IAO_0000114 "needs work" ;
                                        rdfs:label "fan state fast"@en ;
                                        skos:definition "Boolean parameter representing a fast fan speed setting in contrast to the default speed setting."@en .


###  https://w3id.org/pmd/hto/FastCooling
<https://w3id.org/pmd/hto/FastCooling> rdf:type owl:Class ;
                                       rdfs:subClassOf <https://w3id.org/pmd/hto/HeattreatmentMethod> ;
                                       rdfs:comment "Anlagenbedingt."@de ,
                                                    """Schnellkühlung kann z.B. durch erhöhten Kühlwasserdurchfluss erfolgen.
Auch erhöhte Gaskühlung durch ventilation."""@de ,
                                                    "The reason for obsoletion is that the term is not clearly defined and usage has been inconsistent." ;
                                       rdfs:label "fast cooling"@en ;
                                       owl:deprecated "true"^^xsd:boolean ;
                                       skos:definition "Schnellkühlung"@de ,
                                                       "Stark beschleunigte Abkühlung ohne Abschreckmedium."@de .


###  https://w3id.org/pmd/hto/Fluid
<https://w3id.org/pmd/hto/Fluid> rdf:type owl:Class ;
                                 rdfs:subClassOf <https://w3id.org/pmd/hto/Medium> ;
                                 rdfs:label "fluid"@en ;
                                 skos:definition "A substance (such as a liquid or gas) tending to flow or conform to the outline of its container" .


###  https://w3id.org/pmd/hto/FurnaceAtmosphere
<https://w3id.org/pmd/hto/FurnaceAtmosphere> rdf:type owl:Class ;
                                             rdfs:isDefinedBy <https://w3id.org/pmd/hto/> ;
                                             rdfs:label "furnace atmosphere"@en ;
                                             skos:definition "atmosphere type present in retort (vacuum, nitriding, neutral, carburizing)"@en .


###  https://w3id.org/pmd/hto/FurnaceCooling
<https://w3id.org/pmd/hto/FurnaceCooling> rdf:type owl:Class ;
                                          rdfs:subClassOf <https://w3id.org/pmd/hto/HeattreatmentMethod> ;
                                          rdfs:isDefinedBy <https://w3id.org/pmd/hto/> ;
                                          rdfs:label "furnace cooling"@en ;
                                          owl:deprecated "true"^^xsd:boolean ;
                                          skos:definition "free cooling with deactivated heating unit and no additonal cooling by e.g. agitade nitrogene -> furnace cool "@en .


###  https://w3id.org/pmd/hto/HTO_0000000
<https://w3id.org/pmd/hto/HTO_0000000> rdf:type owl:Class ;
                                       rdfs:label "heat treatment elementals"@en .


###  https://w3id.org/pmd/hto/HTO_0000001
<https://w3id.org/pmd/hto/HTO_0000001> rdf:type owl:Class ;
                                       rdfs:label "quenching function"@en ;
                                       skos:definition "A quenching function is a (realizable) function that, when realized, enables a system to lower the temparature of a material fast enough, that it hinders diffusion processes and thus produces metastable material states."@en ,
                                                       "Eine Abschreckfunktion ist eine (realisierbare) Funktion, die es einem System ermöglicht die Temperatur eines Material schnell genug abzusenken, sodass Diffusionsprozesse behindert und dadurch metastabile Materialzustände erzeugt werden."@de ;
                                       skos:example "The function of a oil bath to quench steel after austenitisation so the material transforms into martensite."@en .


###  https://w3id.org/pmd/hto/HTO_0000002
<https://w3id.org/pmd/hto/HTO_0000002> rdf:type owl:Class ;
                                       rdfs:subClassOf [ rdf:type owl:Restriction ;
                                                         owl:onProperty obo:IAO_0000039 ;
                                                         owl:someValuesFrom <https://w3id.org/pmd/hto/HTO_0000010>
                                                       ] ;
                                       rdfs:label "target temperature specification"@en .


###  https://w3id.org/pmd/hto/HTO_0000003
<https://w3id.org/pmd/hto/HTO_0000003> rdf:type owl:Class ;
                                       rdfs:subClassOf [ rdf:type owl:Restriction ;
                                                         owl:onProperty obo:IAO_0000136 ;
                                                         owl:someValuesFrom <https://w3id.org/pmd/hto/HTO_0000005>
                                                       ] ;
                                       rdfs:label "temperature change rate specification"@en ;
                                       skos:definition "Device specification which - as part of plan specifications (e.g. recipes) - specifies the rate at which temparature is to be changed." .


###  https://w3id.org/pmd/hto/HTO_0000004
<https://w3id.org/pmd/hto/HTO_0000004> rdf:type owl:Class ;
                                       rdfs:subClassOf [ owl:intersectionOf ( [ rdf:type owl:Restriction ;
                                                                                owl:onProperty obo:BFO_0000051 ;
                                                                                owl:someValuesFrom <https://w3id.org/pmd/hto/HTO_0000002>
                                                                              ]
                                                                              [ rdf:type owl:Restriction ;
                                                                                owl:onProperty obo:BFO_0000051 ;
                                                                                owl:someValuesFrom <https://w3id.org/pmd/hto/HTO_0000003>
                                                                              ]
                                                                            ) ;
                                                         rdf:type owl:Class
                                                       ] ;
                                       rdfs:label "heating recipe"@en .


###  https://w3id.org/pmd/hto/HTO_0000005
<https://w3id.org/pmd/hto/HTO_0000005> rdf:type owl:Class ;
                                       rdfs:label "temperature change rate"@en ;
                                       skos:definition "A process attribute defining the change of temperature per time unit within a process."@en ;
                                       skos:prefLabel "temperature change rate" .


###  https://w3id.org/pmd/hto/HTO_0000006
<https://w3id.org/pmd/hto/HTO_0000006> rdf:type owl:Class ;
                                       rdfs:label "target temperature"@en ;
                                       skos:definition "Process characteristic defining the temperature that is to be reached within a process that involves a defined change of temperature."@en ;
                                       skos:prefLabel "target temperature"@en .


###  https://w3id.org/pmd/hto/HTO_0000007
<https://w3id.org/pmd/hto/HTO_0000007> rdf:type owl:Class ;
                                       rdfs:label "melting temperature"@en ;
                                       skos:definition "disposition of a material at which a phase transformation between liquid and solid state takes place" .


###  https://w3id.org/pmd/hto/HTO_0000008
<https://w3id.org/pmd/hto/HTO_0000008> rdf:type owl:Class ;
                                       rdfs:subClassOf [ rdf:type owl:Restriction ;
                                                         owl:onProperty obo:IAO_0000136 ;
                                                         owl:someValuesFrom <https://w3id.org/pmd/hto/HTO_0000009>
                                                       ] ;
                                       rdfs:label "duration specification"@en ;
                                       skos:definition "Device specification as part of a plan specification which specifies the duration of a given process." .


###  https://w3id.org/pmd/hto/HTO_0000009
<https://w3id.org/pmd/hto/HTO_0000009> rdf:type owl:Class ;
                                       rdfs:label "duration"@en .


###  https://w3id.org/pmd/hto/HTO_0000010
<https://w3id.org/pmd/hto/HTO_0000010> rdf:type owl:Class ;
                                       rdfs:label "temperature unit"@en .


###  https://w3id.org/pmd/hto/HTO_0000011
<https://w3id.org/pmd/hto/HTO_0000011> rdf:type owl:Class ;
                                       rdfs:comment "needs more work; austenitic phase can be reached from at least two temperatures for any given material (from liquid or from ferrite)" ;
                                       rdfs:label "austenitizing temperature"@en ;
                                       skos:definition "disposition of material which marks the phase change to austenite" .


###  https://w3id.org/pmd/hto/HTO_0000012
<https://w3id.org/pmd/hto/HTO_0000012> rdf:type owl:Class ;
                                       rdfs:label "holding function"@en ;
                                       skos:definition "A holding function is a (realizable) function that, when realized, enables a system or device to hold the thermal energy of a material, typically to facilitate diffusion and phase transformation processes within the material."@en ;
                                       skos:example "function of a furnace to hold its temperature at a specified temperature" .


###  https://w3id.org/pmd/hto/HTO_0000013
<https://w3id.org/pmd/hto/HTO_0000013> rdf:type owl:Class ;
                                       rdfs:subClassOf [ rdf:type owl:Restriction ;
                                                         owl:onProperty obo:BFO_0000051 ;
                                                         owl:someValuesFrom <https://w3id.org/pmd/hto/HTO_0000004>
                                                       ] ,
                                                       [ rdf:type owl:Restriction ;
                                                         owl:onProperty obo:BFO_0000051 ;
                                                         owl:someValuesFrom <https://w3id.org/pmd/hto/HTO_0000014>
                                                       ] ,
                                                       [ rdf:type owl:Restriction ;
                                                         owl:onProperty obo:BFO_0000051 ;
                                                         owl:someValuesFrom <https://w3id.org/pmd/hto/HTO_0000015>
                                                       ] ,
                                                       [ rdf:type owl:Restriction ;
                                                         owl:onProperty obo:BFO_0000051 ;
                                                         owl:someValuesFrom <https://w3id.org/pmd/hto/HTO_0000016>
                                                       ] ;
                                       rdfs:comment "add target temperature in axioms, combine it with austenitisation temperature" ;
                                       rdfs:label "hardening recipe"@en .


###  https://w3id.org/pmd/hto/HTO_0000014
<https://w3id.org/pmd/hto/HTO_0000014> rdf:type owl:Class ;
                                       rdfs:subClassOf [ owl:intersectionOf ( [ rdf:type owl:Restriction ;
                                                                                owl:onProperty obo:BFO_0000051 ;
                                                                                owl:someValuesFrom <https://w3id.org/pmd/hto/HTO_0000002>
                                                                              ]
                                                                              [ rdf:type owl:Restriction ;
                                                                                owl:onProperty obo:BFO_0000051 ;
                                                                                owl:someValuesFrom <https://w3id.org/pmd/hto/HTO_0000008>
                                                                              ]
                                                                            ) ;
                                                         rdf:type owl:Class
                                                       ] ;
                                       rdfs:label "holding recipe"@en .


###  https://w3id.org/pmd/hto/HTO_0000015
<https://w3id.org/pmd/hto/HTO_0000015> rdf:type owl:Class ;
                                       rdfs:subClassOf [ owl:intersectionOf ( [ rdf:type owl:Restriction ;
                                                                                owl:onProperty obo:BFO_0000051 ;
                                                                                owl:someValuesFrom <https://w3id.org/pmd/hto/HTO_0000002>
                                                                              ]
                                                                              [ rdf:type owl:Restriction ;
                                                                                owl:onProperty obo:BFO_0000051 ;
                                                                                owl:someValuesFrom <https://w3id.org/pmd/hto/HTO_0000008>
                                                                              ]
                                                                            ) ;
                                                         rdf:type owl:Class
                                                       ] ;
                                       rdfs:label "soaking recipe"@en .


###  https://w3id.org/pmd/hto/HTO_0000016
<https://w3id.org/pmd/hto/HTO_0000016> rdf:type owl:Class ;
                                       rdfs:subClassOf <https://w3id.org/pmd/hto/HTO_0000017> ;
                                       rdfs:label "quenching recipe"@en .


###  https://w3id.org/pmd/hto/HTO_0000017
<https://w3id.org/pmd/hto/HTO_0000017> rdf:type owl:Class ;
                                       rdfs:label "cooling recipe"@en .


###  https://w3id.org/pmd/hto/HTO_0000018
<https://w3id.org/pmd/hto/HTO_0000018> rdf:type owl:Class ;
                                       rdfs:label "nitriding recipe"@en .


###  https://w3id.org/pmd/hto/HTO_0000019
<https://w3id.org/pmd/hto/HTO_0000019> rdf:type owl:Class ;
                                       rdfs:subClassOf <https://w3id.org/pmd/hto/Hardening> ;
                                       rdfs:label "surface hardening"@en .


###  https://w3id.org/pmd/hto/HTO_0000020
<https://w3id.org/pmd/hto/HTO_0000020> rdf:type owl:Class ;
                                       rdfs:subClassOf <https://w3id.org/pmd/hto/Hardening> ;
                                       rdfs:label "through hardening"@en .


###  https://w3id.org/pmd/hto/HTO_0000021
<https://w3id.org/pmd/hto/HTO_0000021> rdf:type owl:Class ;
                                       rdfs:subClassOf [ rdf:type owl:Restriction ;
                                                         owl:onProperty obo:BFO_0000051 ;
                                                         owl:someValuesFrom <https://w3id.org/pmd/hto/HTO_0000013>
                                                       ] ,
                                                       [ rdf:type owl:Restriction ;
                                                         owl:onProperty obo:BFO_0000051 ;
                                                         owl:someValuesFrom <https://w3id.org/pmd/hto/HTO_0000023>
                                                       ] ;
                                       rdfs:label "QT recipe"@en .


###  https://w3id.org/pmd/hto/HTO_0000022
<https://w3id.org/pmd/hto/HTO_0000022> rdf:type owl:Class ;
                                       rdfs:label "quenching and tempering"@en .


###  https://w3id.org/pmd/hto/HTO_0000023
<https://w3id.org/pmd/hto/HTO_0000023> rdf:type owl:Class ;
                                       rdfs:comment "add target temperature in axioms" ;
                                       rdfs:label "tempering recipe"@en .


###  https://w3id.org/pmd/hto/HTO_0000025
<https://w3id.org/pmd/hto/HTO_0000025> rdf:type owl:Class ;
                                       rdfs:label "carburizing"@en .


###  https://w3id.org/pmd/hto/HTO_0000027
<https://w3id.org/pmd/hto/HTO_0000027> rdf:type owl:Class ;
                                       obo:IAO_0000115 "A process attribute. Describes the pressure set point for a given process."@en ;
                                       rdfs:label "target pressure"@en ;
                                       skos:prefLabel "target pressure"@en .


###  https://w3id.org/pmd/hto/HTO_0000028
<https://w3id.org/pmd/hto/HTO_0000028> rdf:type owl:Class ;
                                       rdfs:subClassOf [ rdf:type owl:Restriction ;
                                                         owl:onProperty obo:RO_0000085 ;
                                                         owl:someValuesFrom <https://w3id.org/pmd/hto/HTO_0000029>
                                                       ] ;
                                       rdfs:label "mass flow controller"@en ;
                                       skos:definition "Device that has the function to control the flow of fluid media to a defined mass flow. It consists of a mass flow meter and a proportional valve."@en .


###  https://w3id.org/pmd/hto/HTO_0000029
<https://w3id.org/pmd/hto/HTO_0000029> rdf:type owl:Class ;
                                       rdfs:label "flow measuring function"@en ;
                                       skos:definition "A subfunction of measuring performed to determine the flow of fluids." .


###  https://w3id.org/pmd/hto/HTO_0000030
<https://w3id.org/pmd/hto/HTO_0000030> rdf:type owl:Class ;
                                       rdfs:subClassOf <https://w3id.org/pmd/hto/HTO_0000005> ;
                                       rdfs:label "heating rate"@en .


###  https://w3id.org/pmd/hto/HTO_0000031
<https://w3id.org/pmd/hto/HTO_0000031> rdf:type owl:Class ;
                                       rdfs:subClassOf <https://w3id.org/pmd/hto/HTO_0000005> ;
                                       rdfs:label "cooling rate"@en .


###  https://w3id.org/pmd/hto/Hardening
<https://w3id.org/pmd/hto/Hardening> rdf:type owl:Class ;
                                     rdfs:isDefinedBy <https://w3id.org/pmd/hto/> ;
                                     rdfs:label "Härten"@de ,
                                                "hardening"@en ;
                                     skos:definition "Heat treatment process with the aim of achieving an increase in strength and hardness of the material."@en ,
                                                     "Wärmebehandlungprozess mit dem Ziel eine Festigkeitssteigerung zu erreichen."@de ;
                                     skos:example """Randschichthärten

Einsatzhärten

Nitrierhärten

verwendet Randschichttiefe""" .


###  https://w3id.org/pmd/hto/HeatingChamber
<https://w3id.org/pmd/hto/HeatingChamber> rdf:type owl:Class ;
                                          rdfs:subClassOf <https://w3id.org/pmd/hto/ChamberScope> ;
                                          rdfs:isDefinedBy <https://w3id.org/pmd/hto/> ;
                                          rdfs:label "Heizkammer"@de ,
                                                     "Ofenkammer mit einer Heizung."@de ,
                                                     "heating chamber"@en ;
                                          skos:definition "Distinguishable chamber of a heat treatment furnace with a heater."@en .


###  https://w3id.org/pmd/hto/HeatingTime
<https://w3id.org/pmd/hto/HeatingTime> rdf:type owl:Class ;
                                       rdfs:isDefinedBy <https://w3id.org/pmd/hto/> ;
                                       rdfs:label "Erwärmdauer"@de ,
                                                  "Heating Time"@en ;
                                       skos:definition "Dauer bis zum Erreichen der Zieltemperatur im Ofen."@de ,
                                                       "Duration until the target temperature is reached in the furnace."@en .


###  https://w3id.org/pmd/hto/HeattreatmentMethod
<https://w3id.org/pmd/hto/HeattreatmentMethod> rdf:type owl:Class ;
                                               obo:IAO_0000114 "needs work" ;
                                               rdfs:comment "The reason for obsoletion is that the term is not clearly defined and usage has been inconsistent." ,
                                                            "all childs are only categories of processes and definatly not roles! what makes a fats cooling? al colling process with some process charateristic on temperature with 100K/min?" ;
                                               owl:deprecated "true"^^xsd:boolean .


###  https://w3id.org/pmd/hto/HeattreatmentScope
<https://w3id.org/pmd/hto/HeattreatmentScope> rdf:type owl:Class ;
                                              obo:IAO_0000114 "needs work" ;
                                              rdfs:comment "childs are processes that realize a certain goal as realizabale" ;
                                              rdfs:isDefinedBy <https://w3id.org/pmd/hto/> ;
                                              rdfs:label "heattreatmentscope"@en ;
                                              owl:deprecated "true"^^xsd:boolean ;
                                              skos:definition "This class specifices the scope of the specific heattreatment process."@en .


###  https://w3id.org/pmd/hto/HydrogeneSensorSignal
<https://w3id.org/pmd/hto/HydrogeneSensorSignal> rdf:type owl:Class ;
                                                 rdfs:comment "nominal pre-set value of control system for hydrogen probe "@en ;
                                                 rdfs:isDefinedBy <https://w3id.org/pmd/hto/> ;
                                                 rdfs:label "hydrogene sensor signal"@en ;
                                                 skos:definition "measured hydrogen value of  hydrogen probe measured in milli volt "@en .


###  https://w3id.org/pmd/hto/LambdaProbeSignal
<https://w3id.org/pmd/hto/LambdaProbeSignal> rdf:type owl:Class ;
                                             rdfs:isDefinedBy <https://w3id.org/pmd/hto/> ;
                                             rdfs:label "lambda probe signal"@en ;
                                             skos:definition "measured lambda probe signal in exhaust gas "@en ,
                                                             "measured signal of the lambda-probe in millivolt, representing the atmospheres redox-potential "@en .


###  https://w3id.org/pmd/hto/LeakageCheck
<https://w3id.org/pmd/hto/LeakageCheck> rdf:type owl:Class ;
                                        rdfs:isDefinedBy <https://w3id.org/pmd/hto/> ;
                                        rdfs:label "leakage check"@en ;
                                        skos:definition "leakage test duration, where the change of pressure after evacuation is rated according to leakages present "@en ,
                                                        "stands for the dwell time during which the pressure increase is evaluated to check tighness of furnace after evacuation initially at process begin "@en .


###  https://w3id.org/pmd/hto/LeakageInterval
<https://w3id.org/pmd/hto/LeakageInterval> rdf:type owl:Class ;
                                           rdfs:comment "Stands for the measurement interval for recording sensor signals (pressure, temperature) and instrument settings (rotational speed, flow rate of MFC), unit as time stamp hh:mm:ss "@en ;
                                           rdfs:isDefinedBy <https://w3id.org/pmd/hto/> ;
                                           rdfs:label "leakage interval"@en ;
                                           skos:definition "effective leakage measuring duration "@en .


###  https://w3id.org/pmd/hto/Medium
<https://w3id.org/pmd/hto/Medium> rdf:type owl:Class ;
                                  obo:IAO_0000114 "needs work" ;
                                  rdfs:comment "no set to be a device specification what to use, but that is not good. medium is a special material entity that has a certain role" ;
                                  rdfs:label "medium"@en ;
                                  skos:definition "A surrounding or enveloping substance" .


###  https://w3id.org/pmd/hto/Nitriding
<https://w3id.org/pmd/hto/Nitriding> rdf:type owl:Class ;
                                     rdfs:isDefinedBy <https://w3id.org/pmd/hto/> ;
                                     rdfs:label "nitriding"@en ;
                                     skos:definition "heat treatment process with the scope to increase the nitrogen content in the surface near area of a sample or part"@en .


###  https://w3id.org/pmd/hto/NitridingDepth
<https://w3id.org/pmd/hto/NitridingDepth> rdf:type owl:Class ;
                                          rdfs:comment "propably some thicknes quality on some special fiat continuent part, diffusion layer having nitrid or something" ;
                                          rdfs:isDefinedBy <https://w3id.org/pmd/hto/> ;
                                          rdfs:label "nitriding depth"@en ;
                                          skos:definition " designated nitriding depth or measured nitriding depth "@en .


###  https://w3id.org/pmd/hto/NitridingPotential
<https://w3id.org/pmd/hto/NitridingPotential> rdf:type owl:Class ;
                                              rdfs:comment "The nitriding potential is a key indicator how intensive the nitriding process is, the higher the value the stronger the nitriding conditions, unit is bar^-3/2"@en ;
                                              rdfs:isDefinedBy <https://w3id.org/pmd/hto/> ;
                                              rdfs:label "nitriding potential"@en ;
                                              skos:definition "calculated nitriding potential, generated out of H2 / NH3 atmosphere content measurement"@en ,
                                                              "nitriding potential of atmosphere calculated from H2 probe signal and ammonia flow rate "@en .


###  https://w3id.org/pmd/hto/OilQuenchingDuration
<https://w3id.org/pmd/hto/OilQuenchingDuration> rdf:type owl:Class ;
                                                rdfs:isDefinedBy <https://w3id.org/pmd/hto/> ;
                                                rdfs:label "Abschreckdauer"@de ,
                                                           "Oil Quenching Duration"@en ;
                                                skos:definition "Dwell time of the components in the quenching medium."@en ,
                                                                "Parameter indicating the duration of the conducted quenching action "@en ,
                                                                "Verweildauer der Bauteile im Abschreckmedium."@de .


###  https://w3id.org/pmd/hto/OverPressure
<https://w3id.org/pmd/hto/OverPressure> rdf:type owl:Class ;
                                        obo:IAO_0000114 "needs work" ;
                                        rdfs:isDefinedBy <https://w3id.org/pmd/hto/> ;
                                        rdfs:label "over pressure"@en ;
                                        skos:definition " Parameter also for liquid or gaseous media for quenching condition of inductive heat treatments, e.g. water pressure or nitrogen pressure in mbar or bar "@en ,
                                                        "Parameter describing a significant higher pressure than ambient pressure, e.g. during a high pressure gas quenching process step, could be mbar or bar "@en .


###  https://w3id.org/pmd/hto/OxygenProbeSignal
<https://w3id.org/pmd/hto/OxygenProbeSignal> rdf:type owl:Class ;
                                             rdfs:isDefinedBy <https://w3id.org/pmd/hto/> ;
                                             rdfs:label "oxygen probe signal"@en ;
                                             skos:definition " measured oxygen probe signal in retort atmosphere "@en .


###  https://w3id.org/pmd/hto/PartialPressure
<https://w3id.org/pmd/hto/PartialPressure> rdf:type owl:Class ;
                                           rdfs:isDefinedBy <https://w3id.org/pmd/hto/> ;
                                           rdfs:label "partial pressure"@en ;
                                           skos:definition " Paramenter describing the intended pressure inside a chamber targeted in a factor relative to one bar (using a vakuum cooling or an atmosphere flow). The complement to vacuum-heating as it allows for active vacuum pump during atmosphere flow. Should be set to zero, if vacuum-heating is true. "@en ,
                                                           "Describing the intended pressure inside a chamber targeted in a factor relative to one bar (using a vakuum cooling or an atmosphere flow)."@en ,
                                                           "Parameter describing the amount of a specific gas species in a mixture, could be mbar "@en ,
                                                           "The complement to vacuum-heating as it allows for active vacuum pump during atmosphere flow. Should be set to zero, if vacuum-heating is true."@en ,
                                                           "nominal pressure of a specific atmosphere component thermochemical steps "@en ,
                                                           "nominal pressure of thermochemical heat treatment pressure during thermochemical steps "@en .


###  https://w3id.org/pmd/hto/QuenchingChamber
<https://w3id.org/pmd/hto/QuenchingChamber> rdf:type owl:Class ;
                                            rdfs:subClassOf <https://w3id.org/pmd/hto/ChamberScope> ;
                                            rdfs:isDefinedBy <https://w3id.org/pmd/hto/> ;
                                            rdfs:label "Abschreckkammer"@de ,
                                                       "Quenching Chamber"@en ;
                                            skos:definition "Chamber of a heat treatment furnace that is designed to quench objects."@en ,
                                                            "Kammer eines Wärmebehandlungsofens, die zum Abschrecken von Gegenständen bestimmt ist."@de .


###  https://w3id.org/pmd/hto/QuenchingLeadtime
<https://w3id.org/pmd/hto/QuenchingLeadtime> rdf:type owl:Class ;
                                             rdfs:isDefinedBy <https://w3id.org/pmd/hto/> ;
                                             rdfs:label "Abschreckvorlaufzeit"@de ,
                                                        "Quenching Leadtime"@en ;
                                             skos:definition "Dauer zwischen Verlassen der Heizkammer und Beginn der effektiven Abschreckung. Gilt für Zweikammeröfen."@de ,
                                                             "Duration between leaving the heating chamber and the start of effective quenching. Applies to two-chamber furnaces."@en ,
                                                             "Parameter indicatin the duration right before the quenching  process "@en .


###  https://w3id.org/pmd/hto/RecordingInterval
<https://w3id.org/pmd/hto/RecordingInterval> rdf:type owl:Class ;
                                             rdfs:comment "stands for the measurement interval for recording sensor signals (pressure, temperature) and instrument settings (rotational speed, flow rate of MFC), unit as time stamp hh:mm:ss "@en ;
                                             rdfs:isDefinedBy <https://w3id.org/pmd/hto/> ;
                                             rdfs:label "recording interval"@en ;
                                             skos:definition " effective data aquisition and saving interval for documentation "@en .


###  https://w3id.org/pmd/hto/Rotation
<https://w3id.org/pmd/hto/Rotation> rdf:type owl:Class ;
                                    obo:IAO_0000114 "needs work" ;
                                    rdfs:comment "seam to be a device specification pinting to a process charateristic of type speed" ;
                                    rdfs:isDefinedBy <https://w3id.org/pmd/hto/> ;
                                    rdfs:label "rotation speed"@en ;
                                    skos:definition " Parameter describing the intended rotational speed of a device as e.g. an fan or turbine, unit revolution per minute. "@en ,
                                                    "rotation speed of the atmosphere agitation device "@en .


###  https://w3id.org/pmd/hto/SequenceDescriptor
<https://w3id.org/pmd/hto/SequenceDescriptor> rdf:type owl:Class ;
                                              rdfs:isDefinedBy <https://w3id.org/pmd/hto/> ;
                                              rdfs:label "sequence descriptor"@en ;
                                              skos:definition "Label of a given process step within a process recipe."@en .


###  https://w3id.org/pmd/hto/SequenceDuration
<https://w3id.org/pmd/hto/SequenceDuration> rdf:type owl:Class ;
                                            rdfs:isDefinedBy <https://w3id.org/pmd/hto/> ;
                                            rdfs:label "sequence duration"@en ;
                                            skos:definition "Duration of a sequence for which certain furnace settings and process parameters can be defined."@en ,
                                                            "Duration of the current heat treatment recipe sequence."@en .


###  https://w3id.org/pmd/hto/SequenceNumber
<https://w3id.org/pmd/hto/SequenceNumber> rdf:type owl:Class ;
                                          rdfs:isDefinedBy <https://w3id.org/pmd/hto/> ;
                                          rdfs:label "sequence number"@en ;
                                          skos:definition " An identifier indicating a process-number in a Workflow represented via consecutive integers "@en ,
                                                          "number of process step of heat treatment recipe "@en ,
                                                          "ongoing number for labeling the process steps within a process recipe "@en .


###  https://w3id.org/pmd/hto/SlowCooling
<https://w3id.org/pmd/hto/SlowCooling> rdf:type owl:Class ;
                                       rdfs:subClassOf <https://w3id.org/pmd/hto/HeattreatmentMethod> ;
                                       rdfs:isDefinedBy <https://w3id.org/pmd/hto/> ;
                                       rdfs:label "Langsame Gleichgewichtsnahabkühlung"@de ,
                                                  "Slow Cooling"@en ;
                                       owl:deprecated "true"^^xsd:boolean ;
                                       skos:definition "Langsame Abkühlung unter gleichgewichtsnahen Bedingungen, um ein gleichgewichtsnahes Gefüge zu erzeugen."@de ,
                                                       "Slow cooling with equilibrium near conditions, to foster an equilibrium near micro structure."@en .


###  https://w3id.org/pmd/hto/SoakingDuration
<https://w3id.org/pmd/hto/SoakingDuration> rdf:type owl:Class ;
                                           rdfs:isDefinedBy <https://w3id.org/pmd/hto/> ;
                                           rdfs:label "Durchwärmzeit"@de ,
                                                      "soaking duration"@en ;
                                           skos:definition "Dauer bis zum Erreichen der homogenen Temperatur im Bauteil."@de ,
                                                           "Duration at isothermal temperatur step."@en ,
                                                           "Duration to achieve a homogenous temperature distribution in the part"@en .


###  https://w3id.org/pmd/hto/SystemTimeForDiagramGeneration
<https://w3id.org/pmd/hto/SystemTimeForDiagramGeneration> rdf:type owl:Class ;
                                                          obo:IAO_0000114 "needs work" ;
                                                          rdfs:comment "usualy a diagram is created out of a process, and it exists then" ;
                                                          rdfs:isDefinedBy <https://w3id.org/pmd/hto/> ;
                                                          rdfs:label "system time for diagram generation"@en ;
                                                          skos:definition " Extrahierte Systemzeit für das Diagram geniert "@de ,
                                                                          "time stamp for measuring data aquisition time and diagram generation / data syncing "@en .


###  https://w3id.org/pmd/hto/Tempering
<https://w3id.org/pmd/hto/Tempering> rdf:type owl:Class ;
                                     obo:IAO_0000114 "needs work"@en ;
                                     rdfs:isDefinedBy <https://w3id.org/pmd/hto/> ;
                                     rdfs:label "Anlassen"@de ,
                                                "tempering"@en ;
                                     skos:definition "A heat treatment process to transform the hardening structure into the direction or equilibrium structure."@en ,
                                                     "Ein Wärmebehandlungsprozess, um das Härtungsgefüge in die Richtung oder in ein Gleichgewichtsgefüge umzuwandeln."@de ,
                                                     "Tempering"@en ,
                                                     "heat treatement process with the scope to reduce the hardness of a prior hardened sample or part"@en .


###  https://w3id.org/pmd/hto/TypeDescription
<https://w3id.org/pmd/hto/TypeDescription> rdf:type owl:Class ;
                                           obo:IAO_0000114 "marked to remove" ;
                                           rdfs:comment "makes no sense to me, if its a decription, create a dc:decription on that individual or class" ;
                                           rdfs:isDefinedBy <https://w3id.org/pmd/hto/> ;
                                           rdfs:label "Typbeschreibung"@de ,
                                                      "Type Description"@en ;
                                           skos:definition "Description for Process Node's utility, e.g. \"Rear Vacuum Furnace Oil Quenching\"."@en .


###  https://w3id.org/pmd/hto/VacuumHeatingPressure
<https://w3id.org/pmd/hto/VacuumHeatingPressure> rdf:type owl:Class ;
                                                 obo:IAO_0000114 "needs work" ;
                                                 rdfs:comment "The reason for obsoletion is that the term is not clearly defined and usage has been inconsistent." ,
                                                              "should be defined as pressur that inheres in a vacum heating pump. Add vacuum heating pump to devices" ;
                                                 rdfs:isDefinedBy <https://w3id.org/pmd/hto/> ;
                                                 rdfs:label "obsolete vacuum heating pressure"@en ;
                                                 owl:deprecated "true"^^xsd:boolean ;
                                                 skos:definition "OBSOLETE. Pressure of the vaccum heating pump."@en .


###  https://w3id.org/pmd/hto/VacuumPressure
<https://w3id.org/pmd/hto/VacuumPressure> rdf:type owl:Class ;
                                          rdfs:comment " in retort measured value of vakuum sensor "@en ,
                                                       " pre-set gas pressure at vacuum sequence "@en ,
                                                       "The reason for obsoletion is that the term is not clearly defined and usage has been inconsistent." ,
                                                       "should be defined in conjuntion to some device or role" ;
                                          rdfs:isDefinedBy <https://w3id.org/pmd/hto/> ;
                                          rdfs:label "obsolete vacuum pressure"@en ;
                                          owl:deprecated "true"^^xsd:boolean ;
                                          skos:definition " Parameter describing the intended vacuum pressure inside a chamber. "@en ,
                                                          "OBSOLETE. Paramenter describing the measured pressure inside a chamber; units could be mbar, bar"@en .


###  https://w3id.org/pmd/hto/cooling
<https://w3id.org/pmd/hto/cooling> rdf:type owl:Class ;
                                   rdfs:subClassOf <https://w3id.org/pmd/hto/HTO_0000000> ,
                                                   [ rdf:type owl:Restriction ;
                                                     owl:onProperty <https://w3id.org/pmd/co/PMD_0000009> ;
                                                     owl:someValuesFrom <https://w3id.org/pmd/hto/HTO_0000005>
                                                   ] ;
                                   rdfs:isDefinedBy <https://w3id.org/pmd/hto/> ;
                                   rdfs:label "Abkühlprozess"@de ,
                                              "cooling"@en ;
                                   skos:definition "A process in which the temperature is lowered from a higher to a lower level."@en ,
                                                   "Ein Prozess, bei dem die Temperatur von einem höherem auf ein niedrigeres Niveau abgesenkt wird."@de .


###  https://w3id.org/pmd/hto/heating
<https://w3id.org/pmd/hto/heating> rdf:type owl:Class ;
                                   rdfs:subClassOf <https://w3id.org/pmd/hto/HTO_0000000> ,
                                                   [ rdf:type owl:Restriction ;
                                                     owl:onProperty <https://w3id.org/pmd/co/PMD_0000009> ;
                                                     owl:someValuesFrom <https://w3id.org/pmd/hto/HTO_0000006>
                                                   ] ;
                                   rdfs:isDefinedBy <https://w3id.org/pmd/hto/> ;
                                   rdfs:label "Erwärmen"@de ,
                                              "heating"@en ;
                                   skos:definition "A process in which the temperature is increased from a lower to a higher level."@en ,
                                                   "Ein Prozess, bei dem die Temperatur von einem niedrigem auf ein höheres Niveau gesteigert wird."@de .


###  https://w3id.org/pmd/hto/holding
<https://w3id.org/pmd/hto/holding> rdf:type owl:Class ;
                                   rdfs:subClassOf <https://w3id.org/pmd/hto/HTO_0000000> ;
                                   rdfs:comment "Die HoldingTime ist stets mit einer vorhergehende SoakingTime verbunden."@de ;
                                   rdfs:isDefinedBy <https://w3id.org/pmd/hto/> ;
                                   rdfs:label "Halten"@de ,
                                              "holding"@en ;
                                   skos:definition "Process step without temperature change in the furnace after the designated temperature was homogeneously reached within the part."@en ,
                                                   "Prozessschritt ohne Temperaturänderung im Ofen."@de .


###  https://w3id.org/pmd/hto/quenching
<https://w3id.org/pmd/hto/quenching> rdf:type owl:Class ;
                                     rdfs:subClassOf <https://w3id.org/pmd/hto/cooling> ;
                                     rdfs:label "Abschrecken"@de ,
                                                "quenching"@en ;
                                     skos:definition "Process with significantly increased cooling rate, aimed at preventing diffusion based transformations."@en ,
                                                     "Prozess mit stark erhöhter Abkühlgeschwindigkeit, mit dem Ziel der Verhinderung diffusionsgesteuerter Umwandlungen."@de .


###  https://w3id.org/pmd/hto/soaking
<https://w3id.org/pmd/hto/soaking> rdf:type owl:Class ;
                                   rdfs:subClassOf <https://w3id.org/pmd/hto/HTO_0000000> ;
                                   rdfs:comment "Durchwärmen des Bauteils, sodass Temperaturhomogenität erreicht wird. Anschließend kann ein Halten auf der Zieltemperatur erfolgen." ;
                                   rdfs:isDefinedBy <https://w3id.org/pmd/hto/> ;
                                   rdfs:label "Durchwärmen"@de ,
                                              "soaking"@en ;
                                   skos:definition "Process step during which temperature homogenization is achieved in the component."@en ,
                                                   "Prozesschritt, während dessen die Temperaturhomogenisierung im Bauteil erreicht wird."@de .


###  Generated by the OWL API (version 4.5.29) https://github.com/owlcs/owlapi
